merge in trunk

acl2svn/branches/centaur/defuns.lisp
@@ -115,49 +115,46 @@
                                           ctx wrld state-vars)))
                    (trans-value (cons x y))))))))))
 
-(defun throw-nonexec-error-p (body)
+(defun chk-non-executable-bodies (names arglists bodies non-executablep ctx
+                                        state)
 
-; We recognize terms that could result from translating (prog2$
-; (throw-nonexec-error 'name ...) ...), i.e., terms of the form
-; (return-last 'progn (throw-non-exec-error ...) ...).
-
-  (and (not (variablep body))
-;      (not (fquotep body))
-       (eq (ffn-symb body) 'return-last)
-       (quotep (fargn body 1))
-       (eq (unquote (fargn body 1)) 'progn)
-       (let ((prog2$-arg1 (fargn body 2)))
-         (and (not (variablep prog2$-arg1))
-;             (not (fquotep prog2$-arg1))
-              (eq (ffn-symb prog2$-arg1)
-                  'throw-nonexec-error)))))
-
-(defun chk-non-executable-bodies (names bodies ctx state)
-
-; Note that bodies are untranslated.
+; Note that bodies are in translated form.
 
   (cond ((endp bodies)
          (value nil))
-        (t (let ((body (car bodies)))
+        (t (let ((name (car names))
+                 (body (car bodies))
+                 (formals (car arglists)))
 
-; Body should be, in essence, (prog2$ (throw-nonexec-error 'name (list
-; . formals)) ...) -- as laid down by defun-nx-fn.  But we do not insist on the
-; use of name and formals in the arguments to throw-nonexec-error, since the
-; choice of those arguments does not affect soundness.
+; The body should be a translated form of (prog2$ (throw-nonexec-error 'name
+; (list . formals)) ...), as laid down by defun-nx-fn.  Normally we insist on
+; the use of name and formals in the arguments to throw-nonexec-error, so that
+; results are as predicted by ev-fncall-rec-logical.  We loosen up that
+; requirement for defproxy, i.e. (eq non-executablep :program), since it won't
+; be true and we don't care that it be true, as we have a program-mode function
+; that does a throw.
 
-             (cond ((throw-nonexec-error-p body)
-                    (chk-non-executable-bodies (cdr names) (cdr bodies) ctx
-                                               state))
+             (cond ((throw-nonexec-error-p body
+                                           (and (not (eq non-executablep
+                                                         :program))
+                                                name)
+                                           formals)
+                    (chk-non-executable-bodies
+                     (cdr names) (cdr arglists) (cdr bodies)
+                     non-executablep ctx state))
                    (t (er soft ctx
                           "The body of a defun that is marked :non-executable ~
                            (perhaps implicitly, by the use of defun-nx) must ~
-                           be of the form (prog2$ (throw-nonexec-error ...).  ~
-                           The definition of ~x0 is thus illegal.  See :DOC ~
-                           defun-nx."
-                          (car names))))))))
+                           be of the form (prog2$ (throw-nonexec-error ...) ~
+                           ...)~@1.  The definition of ~x0 is thus illegal.  ~
+                           See :DOC defun-nx."
+                          (car names)
+                          (if (eq non-executablep :program)
+                              ""
+                            " that is laid down by defun-nx"))))))))
 
-(defun translate-bodies (non-executablep names bodies known-stobjs-lst ctx wrld
-                                         state)
+(defun translate-bodies (non-executablep names arglists bodies known-stobjs-lst
+                                         ctx wrld state)
 
 ; Translate the bodies given and return a pair consisting of their translations
 ; and the final bindings from translate.  Note that non-executable :program
@@ -177,7 +174,8 @@
            (cond (erp ; erp is a ctx, lst is a msg
                   (er soft erp "~@0" lst))
                  (non-executablep
-                  (chk-non-executable-bodies names lst ctx state))
+                  (chk-non-executable-bodies names arglists lst
+                                             non-executablep ctx state))
                  (t (value nil)))
            (cond ((eq non-executablep t)
                   (value (cons lst (pairlis-x2 names '(nil)))))
@@ -5843,9 +5841,10 @@
 ; We determine whether lst is a plausible cdr for a DECLARE form.  Ignoring the
 ; order of presentation and the number of occurrences of each element
 ; (including 0), we ensure that lst is of the form (... (TYPE ...) ... (IGNORE
-; ...) ... (XARGS ... :key val ...) ...)  where the :keys are our xarg keys
-; (members of *xargs-keywords*).
+; ...) ... (IGNORABLE ...) ... (XARGS ... :key val ...) ...)  where the :keys
+; are our xarg keys (members of *xargs-keywords*).
 
+  (declare (xargs :guard t))
   (cond ((atom lst) (null lst))
         ((and (consp (car lst))
               (true-listp (car lst))
@@ -5866,12 +5865,13 @@
 ; functions below.
 
 ; Note: This predicate is not actually used by defuns but is used by
-; verify-termination in order to guard its exploration of the proposed dcls
-; to merge them with the existing ones.  After we define the predicate we
-; define the exploration functions, which implicitly assume this fn as their
-; guard.  The exploration functions below are used in defuns, in particular,
-; in the determination of whether a proposed defun is redundant.
+; verify-termination in order to guard its exploration of the proposed dcls to
+; merge them with the existing ones.  After we define the predicate we define
+; the exploration functions, which assume this fn as their guard.  The
+; exploration functions below are used in defuns, in particular, in the
+; determination of whether a proposed defun is redundant.
 
+  (declare (xargs :guard t))
   (cond ((atom lst) (null lst))
         ((stringp (car lst)) (plausible-dclsp (cdr lst)))
         ((and (consp (car lst))
@@ -5885,7 +5885,8 @@
 ; "fields" used or delete certain fields.
 
 (defun dcl-fields1 (lst)
-  (cond ((null lst) nil)
+  (declare (xargs :guard (plausible-dclsp1 lst)))
+  (cond ((endp lst) nil)
         ((member-eq (caar lst) '(type ignore ignorable))
          (add-to-set-eq (caar lst) (dcl-fields1 (cdr lst))))
         (t (union-eq (evens (cdar lst)) (dcl-fields1 (cdr lst))))))
@@ -5897,7 +5898,8 @@
 ; "field names" used in lst.  Our answer is a subset of the list
 ; *xargs-keywords*.
 
-  (cond ((null lst) nil)
+  (declare (xargs :guard (plausible-dclsp lst)))
+  (cond ((endp lst) nil)
         ((stringp (car lst))
          (add-to-set-eq 'comment (dcl-fields (cdr lst))))
         (t (union-eq (dcl-fields1 (cdar lst))
@@ -5918,6 +5920,8 @@
                        (strip-keyword-list fields (cddr lst)))))))
 
 (defun strip-dcls1 (fields lst)
+  (declare (xargs :guard (and (symbol-listp fields)
+                              (plausible-dclsp1 lst))))
   (cond ((endp lst) nil)
         ((member-eq (caar lst) '(type ignore ignorable))
          (cond ((member-eq (caar lst) fields) (strip-dcls1 fields (cdr lst)))
@@ -5935,6 +5939,8 @@
 ; part of it that specifies a value for one of the fields named.  The result
 ; satisfies plausible-dclsp.
 
+  (declare (xargs :guard (and (symbol-listp fields)
+                              (plausible-dclsp lst))))
   (cond ((endp lst) nil)
         ((stringp (car lst))
          (cond ((member-eq 'comment fields) (strip-dcls fields (cdr lst)))
@@ -5944,18 +5950,9 @@
                    (t (cons (cons 'declare temp)
                             (strip-dcls fields (cdr lst)))))))))
 
-(defun fetch-dcl-field1 (field-name lst)
-  (cond ((null lst) nil)
-        ((member-eq (caar lst) '(type ignore ignorable))
-         (if (eq (caar lst) field-name)
-             (cons (cdar lst) (fetch-dcl-field1 field-name (cdr lst)))
-             (fetch-dcl-field1 field-name (cdr lst))))
-        (t (let ((temp (assoc-keyword field-name (cdar lst))))
-             (cond (temp (cons (cadr temp)
-                               (fetch-dcl-field1 field-name (cdr lst))))
-                   (t (fetch-dcl-field1 field-name (cdr lst))))))))
-
 (defun fetch-dcl-fields2 (field-names kwd-list acc)
+  (declare (xargs :guard (and (symbol-listp field-names)
+                              (keyword-value-listp kwd-list))))
   (cond ((endp kwd-list)
          acc)
         (t (let ((acc (fetch-dcl-fields2 field-names (cddr kwd-list) acc)))
@@ -5964,6 +5961,8 @@
                acc)))))
 
 (defun fetch-dcl-fields1 (field-names lst)
+  (declare (xargs :guard (and (symbol-listp field-names)
+                              (plausible-dclsp1 lst))))
   (cond ((endp lst) nil)
         ((member-eq (caar lst) '(type ignore ignorable))
          (if (member-eq (caar lst) field-names)
@@ -5973,9 +5972,20 @@
                              (fetch-dcl-fields1 field-names (cdr lst))))))
 
 (defun fetch-dcl-fields (field-names lst)
+  (declare (xargs :guard (and (symbol-listp field-names)
+                              (plausible-dclsp lst))))
+  (cond ((endp lst) nil)
+        ((stringp (car lst))
+         (if (member-eq 'comment field-names)
+             (cons (car lst) (fetch-dcl-fields field-names (cdr lst)))
+           (fetch-dcl-fields field-names (cdr lst))))
+        (t (append (fetch-dcl-fields1 field-names (cdar lst))
+                   (fetch-dcl-fields field-names (cdr lst))))))
+
+(defun fetch-dcl-field (field-name lst)
 
 ; Lst satisfies plausible-dclsp, i.e., is the sort of thing you would find
-; between the formals and the body of a DEFUN.  Field-name is one of the
+; between the formals and the body of a DEFUN.  Field-name is 'comment or one of the
 ; symbols in the list *xargs-keywords*.  We return the list of the contents of
 ; all fields with that name.  We assume we will find at most one specification
 ; per XARGS entry for a given keyword.
@@ -5986,15 +5996,8 @@
 ; INTEGER X Y)) then our output will be (... (INTEGER X Y) ...) where the ...
 ; are the other TYPE entries.
 
-  (cond ((endp lst) nil)
-        ((stringp (car lst))
-         (if (member-eq 'comment field-names)
-             (cons (car lst) (fetch-dcl-fields field-names (cdr lst)))
-           (fetch-dcl-fields field-names (cdr lst))))
-        (t (append (fetch-dcl-fields1 field-names (cdar lst))
-                   (fetch-dcl-fields field-names (cdr lst))))))
-
-(defun fetch-dcl-field (field-name lst)
+  (declare (xargs :guard (and (symbolp field-name)
+                              (plausible-dclsp lst))))
   (fetch-dcl-fields (list field-name) lst))
 
 (defun set-equalp-eq (lst1 lst2)
@@ -7763,6 +7766,7 @@
          ((bodies-and-bindings
            (translate-bodies non-executablep ; t or :program
                              names
+                             arglists
                              (get-bodies fives)
                              stobjs-in-lst ; see "slight abuse" comment below
                              ctx wrld2 state)))
@@ -8132,7 +8136,8 @@
   the definitional body has a certain form, we suggest using the macro
   ~c[defun-nx] or ~c[defund-nx]; ~pl[defun-nx].  A third value of
   ~c[:non-executable] for advanced users is ~c[:program], which is generated by
-  expansion of ~c[defproxy] forms; ~pl[defproxy].
+  expansion of ~c[defproxy] forms; ~pl[defproxy].  For another way to deal with
+  non-executability, ~pl[non-exec].
 
   ~c[:NORMALIZE]~nl[]
   Value is a flag telling ~ilc[defun] whether to propagate ~ilc[if] tests
@@ -8770,7 +8775,7 @@
 ; Note: At the moment, defstobj does not introduce any mutually
 ; recursive functions.  So every name is handled separately by
 ; defuns-fns.  Hence, names, here, is always a singleton, though we do
-; not exploit that. Also, embedded-event-lst is always a list
+; not exploit that.  Also, embedded-event-lst is always a list
 ; ee-entries, each being a cons with the name of some superevent like
 ; ENCAPSULATE, INCLUDE-BOOK, or DEFSTOBJ, in the car.  The ee-entry
 ; for the most immediate superevent is the first on the list.  At the
