acl2svn/branches/centaur/axioms.lisp
@@ -5978,6 +5978,103 @@
   (declare (xargs :guard t))
   `(ec-call1 nil ,x))
 
+(defmacro non-exec (x)
+
+  ":Doc-Section ACL2::ACL2-built-ins
+
+  mark code as non-executable~/
+
+  ~c[Non-exec] is a macro such that logically, ~c[(non-exec x)] is equal to
+  ~c[x].  However, the argument to a call of ~c[non-exec] need not obey the
+  usual syntactic restrictions for executable code, and indeed, evaluation of a
+  call of ~c[non-exec] will result in an error.  Moreover, for any form
+  occurring in the body of a function (~pl[defun]) that is a call of
+  ~c[non-exec], no guard proof obligations are generated for that form.
+
+  The following example, although rather contrived, illustrates the use of
+  ~c[non-exec].  One can imagine a less contrived example that efficiently
+  computes return values for a small number of fixed inputs and, for other
+  inputs, returns something logically ``consistent'' with those return values.
+  ~bv[]
+  (defun double (x)
+    (case x
+      (1 2)
+      (2 4)
+      (3 6)
+      (otherwise (non-exec (* 2 x)))))
+  ~ev[]
+  We can prove that ~c[double] is compliant with Common Lisp (~pl[guard]) and
+  that it always computes ~c[(* 2 x)].
+  ~bv[]
+  (verify-guards double)
+  (thm (equal (double x) (* 2 x)))
+  ~ev[]
+  We can evaluate double on the specified arguments.  But a call of
+  ~c[non-exec] results in an error message that reports the form that was
+  supplied to ~c[non-exec].
+  ~bv[]
+  ACL2 !>(double 3)
+  6
+  ACL2 !>(double 10)
+
+
+  ACL2 Error in TOP-LEVEL:  ACL2 has been instructed to cause an error
+  because of an attempt to evaluate the following form (see :DOC non-
+  exec):
+
+    (* 2 X).
+
+  To debug see :DOC print-gv, see :DOC trace, and see :DOC wet.
+
+  ACL2 !>
+  ~ev[]~/
+
+  During proofs, the error is silent; it is ``caught'' by the proof mechanism
+  and generally results in the introduction of a call of ~ilc[hide] during a
+  proof.
+
+  Also ~pl[defun-nx] for a utility that makes every call of a function
+  non-executable, rather than a specified form.  The following examples
+  contrast ~c[non-exec] with ~ilc[defun-nx], in particular illustratating the
+  role of ~ilc[non-exec] in avoiding guard proof obligations.
+  ~bv[]
+  ; Guard verification fails:
+  (defun-nx f1 (x)
+    (declare (xargs :guard t))
+    (car x))
+
+  ; Guard verification succeeds after changing the guard above:
+  (defun-nx f1 (x)
+    (declare (xargs :guard (consp x)))
+    (car x))
+
+  ; Guard verification succeeds:
+  (defun f2 (x)
+    (declare (xargs :guard t))
+    (non-exec (car x)))
+
+  ; Evaluating (g1) prints \"Hello\" before signaling an error.
+  (defun g1 ()
+    (f1 (cw \"Hello\")))
+
+  ; Evaluating (g2) does not print before signaling an error.
+  (defun g2 ()
+    (non-exec (cw \"Hello\")))
+
+  ; Evaluating (h1) gives a guard violation for taking reciprocal of 0.
+  (defun h1 ()
+    (f1 (/ 1 0)))
+
+  ; Evaluating (h2) does not take a reciprocal, hence there is no guard
+  ; violation for that; we just get the error expected from using non-exec.
+  (defun h2 ()
+    (non-exec (/ 0)))
+  ~ev[]"
+
+  (declare (xargs :guard t))
+  `(prog2$ (throw-nonexec-error :non-exec ',x)
+           ,x))
+
 #+acl2-loop-only
 (defmacro / (x &optional (y 'nil binary-casep))
 
@@ -7697,10 +7794,9 @@
   ~c[(not (eq op 'SKIP))] are tau predicates.  The tau system recognizes several
   variants of ~ilc[EQUAL].
 
-  The tau algorithm is a decision procedure for the logical theory described (only)
-  by the rules in the data base.  The decision procedure can be enabled or
-  disabled.  It is disabled by default, for backwards compability with the books
-  in ACL2's regression suite.
+  The tau algorithm is a decision procedure for the logical theory
+  described (only) by the rules in the data base.  The decision procedure can
+  be enabled or disabled.  It is enabled by default.
 
   The data base contains rules derived from theorems stated by the user.
   Unlike a type system, the tau system cannot automatically infer relations
@@ -7809,18 +7905,19 @@
   (implies (and (p1 v) ... (pk v)) (q v)), ; Here k must exceed 1.
 
   ~i[Signature Form 1]:
-  (implies (and (p1 x1) (p2 x2) ...)       ; See Note below
+  (implies (and (p1 x1) (p2 x2) ...)       ; See Note below.
            (q (fn x1 x2 ...)))
 
   ~i[Signature Form 2]:
-  (implies (and (p1 x1) (p2 x2) ...)       ; See Note below
+  (implies (and (p1 x1) (p2 x2) ...)       ; See Note below.
            (q (mv-nth 'n (fn x1 x2 ...))))
 
   ~i[Big Switch]:
-  (equal (fn . formals) body),              ; See Note below.
+  (equal (fn . formals) body),             ; See Note below.
 
-  ~i[MV-NTH Synonym]:
-  (equal (fn x y) (mv-nth x y))
+  ~i[MV-NTH Synonym]:                          ; Extend Signature Form 2 to
+  (equal (nth-alt x y) (mv-nth x y)) or    ; apply not only to mv-nth, but when
+  (equal (mv-nth x y) (nth-alt x y))       ; mv-nth is replaced by nth-alt.
   ~ev[]
 
   Note on the Boolean Form: When a ~c[:tau-system] rule of this form is proved,
@@ -7845,6 +7942,8 @@
   expression in which a variable is compared successively to a sequence of
   symbols.  Only the ~i[first] big switch equation for a given function symbol
   ~c[fn] is stored!
+
+  Note on the MV-NTH Synonym Forms: These forms 
 
   To see what the tau system ``knows'' about a given function symbol
   ~pl[tau-data].  To see the entire tau data base, ~pl[tau-data-base].
@@ -12334,7 +12433,20 @@
 ; Begin support for defun-nx.
 
 (defun throw-nonexec-error (fn actuals)
-  (declare (xargs :guard t
+  (declare (xargs :guard
+
+; An appropriate guard would seem to be the following.
+
+;                 (if (keywordp fn)
+;                     (eq fn :non-exec)
+;                   (and (symbolp fn)
+;                        (true-listp actuals)))
+
+; However, we want to be sure that the raw Lisp code is evaluated even if
+; guard-checking has been set to :none.  A simple fix is to replace the actuals
+; if they are ill-formed, and that is what we do.
+
+                  t
                   :verify-guards nil)
            #+acl2-loop-only
            (ignore fn actuals))
@@ -12351,7 +12463,13 @@
 
             nil
             fn
-            (print-list-without-stobj-arrays actuals)))
+            (if (eq fn :non-exec)
+                actuals
+              (print-list-without-stobj-arrays
+               (if (true-listp actuals)
+                   actuals
+                 (error "Unexpected case: Ill-formed actuals for ~
+                         throw-nonexec-error!"))))))
 
 ; Just in case throw-raw-ev-fncall doesn't throw -- though it always should.
 
@@ -12398,9 +12516,11 @@
   single-threadedness (~pl[stobj]) and multiple-values passing (~pl[mv] and
   ~pl[mv-let]).  After such a definition is admitted, the usual syntactic rules
   for ~ilc[state] and user-defined ~il[stobj]s are relaxed for calls of the
-  function it defines.
+  function it defines.  Also ~pl[non-exec] for a way to designate subterms of
+  function bodies, or subterms of code to be executed at the top level, as
+  non-executable.
 
-  The syntax is identical to that of ~ilc[defun].  A form
+  The syntax of ~c[defun-nx] is identical to that of ~ilc[defun].  A form
   ~bv[]
   (defun-nx name (x1 ... xk) ... body)
   ~ev[]
@@ -12414,14 +12534,6 @@
   ~ev[]
   Note that because of the insertion of the above call of
   ~c[throw-nonexec-error], no formal is ignored when using ~c[defun-nx].~/
-
-  If you prefer to avoid the use of ~c[defun-nx] for non-executable function
-  definitions in ~c[:]~ilc[logic] mode, you can use an ~ilc[xargs]
-  ~c[:non-executable t] ~ilc[declare] form, provided the body has the form
-  ~c[(prog2$ (throw-nonexec-error ...) ...)].  The function
-  ~c[throw-nonexec-error] is guaranteed to cause an error, though the
-  ~c[:non-executable] keyword will lay down code such that an error generally
-  occurs when calling ~c[name] without calling ~c[throw-nonexec-error].
 
   During proofs, the error is silent; it is ``caught'' by the proof mechanism
   and generally results in the introduction of a call of ~ilc[hide] during a
@@ -12439,6 +12551,13 @@
   Note that ~c[defund-nx] is also available.  It has an effect identical to
   that of ~c[defun-nx] except that as with ~ilc[defund], it leaves the function
   disabled.
+
+  If you use guards (~pl[guard]), please be aware that even though syntactic
+  restrictions are relaxed for ~c[defun-nx], guard verification proceeds
+  exactly as for ~ilc[defun].  If you want ACL2 to skip a form for purposes of
+  generating guard proof obligations, use the macro ~ilc[non-exec], which
+  generates a call of ~c[throw-nonexec-error] that differs somewhat from the
+  one displayed above.  ~l[non-exec].
 
   ~l[defun] for documentation of ~c[defun]."
 
@@ -12839,6 +12958,12 @@
   (and (consp x)
        (eq (car x) 'quote)))
 
+(defconst *t* (quote (quote t)))
+(defconst *nil* (quote (quote nil)))
+(defconst *0* (quote (quote 0)))
+(defconst *1* (quote (quote 1)))
+(defconst *-1* (quote (quote -1)))
+
 (defun kwote (x)
 
   ":Doc-Section ACL2::ACL2-built-ins
@@ -12852,7 +12977,21 @@
   To see the ACL2 definition of this function, ~pl[pf].~/~/"
 
   (declare (xargs :guard t))
-  (list 'quote x))
+  (mbe :logic
+
+; Theorem ev-lambda-clause-correct in
+; books/centaur/misc/evaluator-metatheorems.lisp goes out to lunch if we use
+; the :exec term below as the definition.  So we keep the :logic definition
+; simple.
+
+       (list 'quote x)
+       :exec ; save conses
+       (cond ((eq x nil) *nil*)
+             ((eq x t) *t*)
+             ((eql x 0) *0*)
+             ((eql x 1) *1*)
+             ((eql x -1) *-1*)
+             (t (list 'quote x)))))
 
 (defun kwote-lst (lst)
 
@@ -13884,6 +14023,14 @@
         (list 'quote r)
         'state))
 
+#+(and :non-standard-analysis (not acl2-loop-only))
+(defun floor1 (x)
+
+; See "RAG" comment in the definition of floor for an explanation of why we
+; need this function.
+
+  (floor x 1))
+
 #+acl2-loop-only
 (progn
 
@@ -13926,6 +14073,8 @@
   interested in learning more about ACL2(r).  Gamboa's dissertation
   may also be helpful.~/")
 
+(defun floor (i j)
+
 ;; RAG - This function had to be modified in a major way.  It was
 ;; originally defined only for rationals, and it used the fact that
 ;; the floor of "p/q" could be found by repeatedly subtracting "q"
@@ -13936,8 +14085,6 @@
 ;; equal to it or smaller to it by no more than 1.  Using this
 ;; function, we can define the more general floor function offered
 ;; below.
-
-(defun floor (i j)
 
   ":Doc-Section ACL2::ACL2-built-ins
 
@@ -16348,8 +16495,10 @@
     (value-triple '(:defund NAME))).
   ~ev[]
   Only the ~c[:]~ilc[definition] rule (and, for recursively defined functions,
-  the ~c[:]~ilc[induction] rule) for the function are disabled, and the summary
-  for the ~ilc[in-theory] event is suppressed.
+  the ~c[:]~ilc[induction] rule) for the function are disabled.  In particular,
+  ~c[defund] does not disable either the ~c[:]~ilc[type-prescription] or the
+  ~c[:]~ilc[executable-counterpart] rule.  Also, the summary for the
+  ~ilc[in-theory] event is suppressed.
 
   Note that ~c[defund] commands are never redundant (~pl[redundant-events]).
   If the function has already been defined, then the ~ilc[in-theory] event
@@ -27791,7 +27940,7 @@
 ; enforces the rule that a function may receive STATE only in a slot
 ; whose STOBJS-IN flag is STATE.  And, with only one exception, the
 ; STOBJS-IN setting is always calculated by noting which formal is
-; called STATE.  So by giving written-files ST and never reseting its
+; called STATE.  So by giving written-files ST and never resetting its
 ; STOBJS-IN, we prevent it from being fed the live state (or any
 ; state) in code (such as defuns and top-level commands) where we are
 ; checking the use of state.  (In theorems, anything goes.)  As noted,
@@ -27843,7 +27992,7 @@
 ; states but which (b) can only be logically defined in terms of calls
 ; to the primitive state accessors and updaters are (i) defined with
 ; STATE-STATE as a formal parameter, (ii) have their property list
-; smashed appropriately for STOBJS-IN and STOBJS-OUT right right after
+; smashed appropriately for STOBJS-IN and STOBJS-OUT right after
 ; their admission, to reflect their true state character, and (iii)
 ; are operationally defined with raw lisp at some level between the
 ; defun and the use of the primitive state accessors and updaters.
@@ -39549,16 +39698,16 @@
   Automatic mode just means that some ~c[:tau-system] rules may be created
   also.
 
-  Of course, if the tau system is in automatic mode and a ~c[defthm] event
-  explicitly specifies a ~c[:tau-system] rule class, that tau rule is created
-  from the proved formula (or the specified ~c[:corollary]) or else an error is
-  caused.  But if the tau system is in automatic mode and a ~c[defthm] event
-  explicitly creates other classes of rules, the system quietly checks whether
-  the formula can be stored as a tau rule and stores it that way if possible,
-  in addition to the specified ways.  It is the shape of the proved formula --
-  not some ~c[:corollary] of some non-~c[:tau-system] rule class -- that
-  determines whether a tau rule is generated.  Of course, no error is signalled
-  if a proved formula of some non-~c[:tau-system] rule class fails to be of an
+  Of course, if a ~c[defthm] event explicitly specifies a ~c[:tau-system] rule
+  class, then even if the tau system is in automatic mode, that tau rule is
+  created from the proved formula (or the specified ~c[:corollary]) or else an
+  error is caused.  But if the tau system is in automatic mode and a ~c[defthm]
+  event doesn't explicitly specify a ~c[:tau-system] rule class, then the
+  system quietly checks each specified ~c[:corollary] ~-[] or, in the absence
+  of any ~c[:corollary], it checks the proved formula ~-[] for whether it can
+  be stored as a tau rule.  If so, then the system stores a tau rule, in
+  addition to storing the specified rule.  Of course, no error is signalled if
+  a proved formula of some non-~c[:tau-system] rule class fails to be of an
   appropriate shape for the tau system.
 
   Recall that the use of tau rules is controlled by the rune
@@ -44428,10 +44577,6 @@ Lisp definition."
 
     (return-from mod-expt (si::powm base exp mod)))
   (mod (expt base exp) mod))
-
-(defconst *t* (quote (quote t)))
-
-(defconst *nil* (quote (quote nil)))
 
 (defmacro fcons-term* (&rest x)
 
